src/parity/direct_parity.lean
@@ -1,6 +1,6 @@
 /-
 This file defines and proves the correctness of the direct (or naive)
-encoding of the n-variable boolean XOR constraint.
+encoding of the n-variable boolean parity constraint.
 
 Authors: Cayden Codel, Jeremy Avigad, Marijn Heule
 Carnegie Mellon University
@@ -33,22 +33,22 @@ variables {l : list (literal V)} {c : clause V}
 
 /- The direct encoding is the set of all possible clauses with an even number 
    of negations on the provided literals in a single CNF formula. -/
-def direct_xor' : list (literal V) → cnf V
+def direct_parity' : list (literal V) → cnf V
 | []        := [[]]
 | (l :: ls) := (explode (map var ls)).map 
       (λ c, ite (!bodd (c.count_flips ls)) (l :: c) (l.flip :: c))
 
 -- Translated into an encoding type
-def direct_xor : enc_fn V := dir_enc direct_xor'
+def direct_parity : enc_fn V := dir_enc direct_parity'
 
-@[simp] theorem direct_xor_nil : direct_xor' ([] : list (literal V)) = [[]] := rfl
-@[simp] theorem direct_xor_singleton (lit : literal V) : direct_xor' [lit] = [[lit]] := rfl
+@[simp] theorem direct_parity_nil : direct_parity' ([] : list (literal V)) = [[]] := rfl
+@[simp] theorem direct_parity_singleton (lit : literal V) : direct_parity' [lit] = [[lit]] := rfl
 
-theorem mem_explode_of_mem_direct_xor : c ∈ direct_xor' l → c ∈ explode (map var l) :=
+theorem mem_explode_of_mem_direct_parity : c ∈ direct_parity' l → c ∈ explode (map var l) :=
 begin
   cases l with l ls,
-  { simp only [explode_nil, imp_self, direct_xor_nil, map_nil] },
-  { simp [direct_xor', explode],
+  { simp only [explode_nil, imp_self, direct_parity_nil, map_nil] },
+  { simp [direct_parity', explode],
     intros cl hcl,
     cases l,
     { cases (bodd (cl.count_flips ls)),
@@ -61,31 +61,31 @@ begin
         use [cl, hcl, h] } } }
 end
 
-theorem length_direct_xor : l ≠ [] → length (direct_xor' l) = 2^(length l - 1) :=
+theorem length_direct_parity : l ≠ [] → length (direct_parity' l) = 2^(length l - 1) :=
 begin
   cases l,
   { contradiction },
-  { simp only [direct_xor', length_explode, add_zero, length, add_succ_sub_one, 
+  { simp only [direct_parity', length_explode, add_zero, length, add_succ_sub_one, 
       ne.def, forall_true_left, not_false_iff, length_map] }
 end
 
-theorem length_direct_xor_pos : l ≠ [] → length (direct_xor' l) > 0 :=
-assume h, by simp only [length_direct_xor h, succ_pos', gt_iff_lt, pow_pos]
+theorem length_direct_parity_pos : l ≠ [] → length (direct_parity' l) > 0 :=
+assume h, by simp only [length_direct_parity h, succ_pos', gt_iff_lt, pow_pos]
 
-theorem exists_mem_direct_xor (l : list (literal V)) : ∃ (c : clause V), c ∈ direct_xor' l :=
+theorem exists_mem_direct_parity (l : list (literal V)) : ∃ (c : clause V), c ∈ direct_parity' l :=
 begin
   cases l with l ls,
   { use [nil, mem_singleton_self nil] },
-  { exact exists_mem_of_length_pos (length_direct_xor_pos (cons_ne_nil l ls)) }
+  { exact exists_mem_of_length_pos (length_direct_parity_pos (cons_ne_nil l ls)) }
 end
 
 -- These theorems begin to be dependent on order of encoding
 -- If the underlying type of parity changes to (fin)set, must update
-theorem map_var_eq_of_mem_direct_xor : c ∈ direct_xor' l → map var c = map var l :=
+theorem map_var_eq_of_mem_direct_parity : c ∈ direct_parity' l → map var c = map var l :=
 begin
   cases l with l ls,
-  { simp only [direct_xor', imp_self, map_eq_nil, map_nil, mem_singleton] },
-  { simp [direct_xor'],
+  { simp only [direct_parity', imp_self, map_eq_nil, map_nil, mem_singleton] },
+  { simp [direct_parity'],
     intros c hc,
     cases (bodd (c.count_flips ls)),
     { simp only [if_true, eq_self_iff_true],
@@ -96,15 +96,15 @@ begin
       simp [map_var_eq_iff_mem_explode.mpr hc, flip_var_eq] } }
 end
 
-theorem even_flips_iff_mem_direct_xor_of_map_var_eq : map var c = map var l → 
-  (bodd (c.count_flips l) = ff ↔ c ∈ direct_xor' l) :=
+theorem even_flips_iff_mem_direct_parity_of_map_var_eq : map var c = map var l → 
+  (bodd (c.count_flips l) = ff ↔ c ∈ direct_parity' l) :=
 begin
   intro hc,
   cases l with l ls,
   { rw [map_nil, map_eq_nil] at hc, subst hc,
-    simp only [count_flips_self, bodd_zero, eq_self_iff_true, direct_xor_nil, mem_singleton] }, 
+    simp only [count_flips_self, bodd_zero, eq_self_iff_true, direct_parity_nil, mem_singleton] }, 
   { split,
-    { simp only [direct_xor', map_cons, bool.cond_to_bool, mem_map],
+    { simp only [direct_parity', map_cons, bool.cond_to_bool, mem_map],
       intro hf,
       rcases exists_cons_of_map_cons hc with ⟨x, xs, rfl, hx, hxs⟩,
       use xs, split,
@@ -118,7 +118,7 @@ begin
           { simp [clause.count_flips, hx] at hf,
             rw h at hf, contradiction },
           { simp only [flip_flip, bool.bnot_tt, coe_sort_ff, if_false]} } } },
-    { { simp only [direct_xor', bool.cond_to_bool, mem_map],
+    { { simp only [direct_parity', bool.cond_to_bool, mem_map],
         rintro ⟨a, ha, hf⟩,
         rcases exists_cons_of_map_cons hc with ⟨x, xs, rfl, hx, hxs⟩,
         cases h : (nat.bodd (a.count_flips ls));
@@ -126,31 +126,31 @@ begin
           simp [← hf, clause.count_flips, literal.is_neg, bool.to_nat, h, flip_flip _, flip_ne] } } } }
 end
 
-theorem odd_flips_iff_not_mem_direct_xor_of_map_var_eq : map var c = map var l → 
-  (bodd (c.count_flips l) = tt ↔ c ∉ direct_xor' l) :=
+theorem odd_flips_iff_not_mem_direct_parity_of_map_var_eq : map var c = map var l → 
+  (bodd (c.count_flips l) = tt ↔ c ∉ direct_parity' l) :=
 begin
   intro hc, split,
   { intro hcount, by_contradiction,
-    rw (even_flips_iff_mem_direct_xor_of_map_var_eq hc).mpr h at hcount,
+    rw (even_flips_iff_mem_direct_parity_of_map_var_eq hc).mpr h at hcount,
     contradiction },
   { contrapose, simp only [eq_ff_eq_not_eq_tt, not_not],
-    exact (even_flips_iff_mem_direct_xor_of_map_var_eq hc).mp }
+    exact (even_flips_iff_mem_direct_parity_of_map_var_eq hc).mp }
 end
 
-theorem mem_direct_xor_self (l : list (literal V)) : l ∈ (direct_xor' l) :=
+theorem mem_direct_parity_self (l : list (literal V)) : l ∈ (direct_parity' l) :=
 begin
   have hcount := clause.count_flips_self l,
   have := nat.bodd_zero,
   rw ← hcount at this,
-  exact (even_flips_iff_mem_direct_xor_of_map_var_eq (refl _)).mp this
+  exact (even_flips_iff_mem_direct_parity_of_map_var_eq (refl _)).mp this
 end
 
--- Some proofs require the stronger statement that direct is exactly xor
-theorem eval_direct_xor_eq_eval_parity (l : list (literal V)) (τ : assignment V) :
-  (direct_xor' l).eval τ = parity.eval τ l :=
+-- Some proofs require the stronger statement that direct is exactly parity
+theorem eval_direct_parity_eq_eval_parity (l : list (literal V)) (τ : assignment V) :
+  (direct_parity' l).eval τ = parity.eval τ l :=
 begin
   cases l with l ls,
-  { simp only [cnf.eval_singleton, eval_nil, direct_xor_nil, clause.eval_nil] },
+  { simp only [cnf.eval_singleton, eval_nil, direct_parity_nil, clause.eval_nil] },
   { have he := eval_eq_bodd_count_tt τ (l :: ls),
     cases h : (parity.eval τ (l :: ls)),
     { apply eval_ff_iff_exists_clause_eval_ff.mpr,
@@ -158,7 +158,7 @@ begin
       split,
       { rw [← clause.count_flips_falsify_eq_count_tt τ (l :: ls),
             clause.count_flips_comm] at he,
-        apply (even_flips_iff_mem_direct_xor_of_map_var_eq 
+        apply (even_flips_iff_mem_direct_parity_of_map_var_eq 
           (clause.falsify_map_var_eq τ (map var (l :: ls)))).mp,
         rw ← h,
         exact he.symm },
@@ -166,57 +166,57 @@ begin
     { rw h at he,
       apply eval_tt_iff_forall_clause_eval_tt.mpr,
       intros c hc,
-      have mve := map_var_eq_of_mem_direct_xor hc,
+      have mve := map_var_eq_of_mem_direct_parity hc,
       have nagree_ond := ne_of_eq_ff_of_eq_tt
-        ((even_flips_iff_mem_direct_xor_of_map_var_eq mve).mpr hc) he.symm,
+        ((even_flips_iff_mem_direct_parity_of_map_var_eq mve).mpr hc) he.symm,
       have neq := ne_of_apply_ne nat.bodd nagree_ond,
       rw clause.count_flips_comm at neq,
       exact clause.eval_tt_of_ne_flips mve.symm (ne.symm neq) } }
 end
 
 -- Formal proof of correctness, see encoding.lean
-theorem direct_xor_formula_encodes_parity (l : list (literal V)) :
-  formula_encodes parity (direct_xor' l) l :=
+theorem direct_parity_formula_encodes_parity (l : list (literal V)) :
+  formula_encodes parity (direct_parity' l) l :=
 begin
   intro τ,
   split,
   { intro h,
     use τ,
-    rw eval_direct_xor_eq_eval_parity l τ,
+    rw eval_direct_parity_eq_eval_parity l τ,
     exact ⟨h, assignment.agree_on.refl τ _⟩ },
   { rintros ⟨σ, he, hs⟩,
-    rw [eval_eq_of_agree_on hs, ← eval_direct_xor_eq_eval_parity l σ],
+    rw [eval_eq_of_agree_on hs, ← eval_direct_parity_eq_eval_parity l σ],
     exact he }
 end
 
-theorem direct_xor_eq_direct_xor (l : list (literal V)) (g : gensym V) :
-  direct_xor' l = (direct_xor l g).1 := rfl
+theorem direct_parity_eq_direct_parity (l : list (literal V)) (g : gensym V) :
+  direct_parity' l = (direct_parity l g).1 := rfl
 
-theorem vars_direct_xor (l : list (literal V)) : 
-  (direct_xor' l).vars = clause.vars l :=
+theorem vars_direct_parity (l : list (literal V)) : 
+  (direct_parity' l).vars = clause.vars l :=
 begin
   cases l with l ls,
-  { simp only [cnf.vars_singleton, direct_xor_nil] },
+  { simp only [cnf.vars_singleton, direct_parity_nil] },
   { rw finset.ext_iff, intro v, split,
     { intro hv,
       rcases mem_vars_iff_exists_mem_clause_and_mem.mp hv with ⟨c, hc⟩,
       rw [clause.mem_vars_iff_mem_map_vars],
-      rw ← (map_var_eq_of_mem_direct_xor hc.1),
+      rw ← (map_var_eq_of_mem_direct_parity hc.1),
       exact clause.mem_vars_iff_mem_map_vars.mp hc.2 },
     { intro hv,
       apply mem_vars_iff_exists_mem_clause_and_mem.mpr,
       use (l :: ls),
-      exact ⟨mem_direct_xor_self _, hv⟩ } }
+      exact ⟨mem_direct_parity_self _, hv⟩ } }
 end
 
-theorem direct_xor_encodes_parity : encodes parity (direct_xor : enc_fn V) :=
+theorem direct_parity_encodes_parity : encodes parity (direct_parity : enc_fn V) :=
 begin
   split,
   { intros l g hdis,
-    rw ← direct_xor_eq_direct_xor,
-    exact direct_xor_formula_encodes_parity l },
+    rw ← direct_parity_eq_direct_parity,
+    exact direct_parity_formula_encodes_parity l },
   { intros l g hdis,
-    simp [direct_xor, dir_enc, vars_direct_xor] }
+    simp [direct_parity, dir_enc, vars_direct_parity] }
 end
 
 end direct_encoding
